Isabelle/Shelley/Properties.thy
@@ -749,54 +749,52 @@ qed
 \<comment> \<open>NOTE: Lemma 15.9 in the spec.\<close>
 \<comment> \<open>NOTE: We require \<open>addr_rwd\<close> to be monotonic, which is a minor (though sensible) deviation from
 the spec.\<close>
-lemma reward_update_value_preservation:
-  assumes "inj addr_rwd"
+lemma reward_update_application_value_preservation:
+  assumes "ru = (\<Delta>t, \<Delta>r, rs, \<Delta>f, i\<^sub>r\<^sub>w\<^sub>d)"
+  and "i\<^sub>r\<^sub>w\<^sub>d = get_ir es"
+  and "\<Delta>f = - get_fee_ss es"
+  and "rewards\<^sub>m\<^sub>i\<^sub>r = (\<Sum> k \<in> fmdom' i\<^sub>r\<^sub>w\<^sub>d. i\<^sub>r\<^sub>w\<^sub>d $$! k)"
+  and "- \<Delta>r = \<Delta>r\<^sub>l + rewards\<^sub>m\<^sub>i\<^sub>r"
+  and "\<Delta>t - \<Delta>r\<^sub>l + (\<Sum> k \<in> fmdom' rs. rs $$! k) + \<Delta>f = 0"
+  and "inj addr_rwd"
   and "mono addr_rwd"
-  shows "val_epoch_state s\<^sub>2 = val_epoch_state (apply_r_upd (create_r_upd b s\<^sub>1) s\<^sub>2)"
+  shows "val_epoch_state es = val_epoch_state (apply_r_upd ru es)"
 proof -
-  obtain treasury\<^sub>1 reserves\<^sub>1 ss\<^sub>1 utxo\<^sub>1 deps\<^sub>1 fees\<^sub>1 up\<^sub>1 stk_creds\<^sub>1 rewards\<^sub>1 i\<^sub>r\<^sub>w\<^sub>d pstate\<^sub>1 ppm\<^sub>1
-    where f0: "s\<^sub>1 =
-      (
-        (treasury\<^sub>1, reserves\<^sub>1),
-        ss\<^sub>1,
-        ((utxo\<^sub>1, deps\<^sub>1, fees\<^sub>1, up\<^sub>1), ((stk_creds\<^sub>1, rewards\<^sub>1, i\<^sub>r\<^sub>w\<^sub>d), pstate\<^sub>1)),
-        ppm\<^sub>1
-      )"
-    by (metis old.prod.exhaust val_deleg_state.cases)
-  then obtain \<Delta>t \<Delta>r rs \<Delta>f where f1: "create_r_upd b s\<^sub>1 = (\<Delta>t, \<Delta>r, rs, \<Delta>f, i\<^sub>r\<^sub>w\<^sub>d)"
-    unfolding Let_def using create_r_upd.elims and get_ir.simps by metis
-  moreover obtain treasury reserves ss utxo deps fees up stk_creds rewards i'\<^sub>r\<^sub>w\<^sub>d pstate ppm
-    where f2: "s\<^sub>2 =
+  obtain treasury reserves pstake\<^sub>m\<^sub>a\<^sub>r\<^sub>k pstake\<^sub>s\<^sub>e\<^sub>t pstake\<^sub>g\<^sub>o pools_ss fee_ss utxo deps fees up stk_creds
+    rewards i'\<^sub>r\<^sub>w\<^sub>d pstate pp
+    where f0: "es =
       (
         (treasury, reserves),
-        ss,
+        (pstake\<^sub>m\<^sub>a\<^sub>r\<^sub>k, pstake\<^sub>s\<^sub>e\<^sub>t, pstake\<^sub>g\<^sub>o, pools_ss, fee_ss),
         ((utxo, deps, fees, up), ((stk_creds, rewards, i'\<^sub>r\<^sub>w\<^sub>d), pstate)),
-        ppm
+        pp
       )"
     by (metis old.prod.exhaust val_deleg_state.cases)
-  ultimately obtain non_distributed and rew'\<^sub>m\<^sub>i\<^sub>r and update\<^sub>r\<^sub>w\<^sub>d and unregistered
-    where f3: "apply_r_upd (\<Delta>t, \<Delta>r, rs, \<Delta>f, i\<^sub>r\<^sub>w\<^sub>d) s\<^sub>2 =
+  with assms(2,3) have "i'\<^sub>r\<^sub>w\<^sub>d = i\<^sub>r\<^sub>w\<^sub>d" and "- fee_ss = \<Delta>f"
+    by (simp, simp)
+  from assms(1,2,4) and f0 obtain non_distributed and rew'\<^sub>m\<^sub>i\<^sub>r and update\<^sub>r\<^sub>w\<^sub>d and unregistered
+    where f1: "apply_r_upd ru es =
       (
         (treasury + \<Delta>t, reserves + \<Delta>r + non_distributed),
-        ss,
+        (pstake\<^sub>m\<^sub>a\<^sub>r\<^sub>k, pstake\<^sub>s\<^sub>e\<^sub>t, pstake\<^sub>g\<^sub>o, pools_ss, fee_ss),
         ((utxo, deps, fees + \<Delta>f, up), ((stk_creds, (rewards \<union>\<^sub>+ rs) \<union>\<^sub>+ update\<^sub>r\<^sub>w\<^sub>d, {$$}), pstate)),
-        ppm
+        pp
       )"
-      and f7: "unregistered = fmdom' stk_creds \<lhd>/ i\<^sub>r\<^sub>w\<^sub>d"
-      and f4: "non_distributed = (\<Sum>k \<in> fmdom' unregistered. unregistered $$! k)"
-      and f5: "rew'\<^sub>m\<^sub>i\<^sub>r = fmdom' stk_creds \<lhd> i\<^sub>r\<^sub>w\<^sub>d"
-      and f6: "update\<^sub>r\<^sub>w\<^sub>d = fmap_of_list [(addr_rwd hk, val). (hk, val) \<leftarrow> sorted_list_of_fmap rew'\<^sub>m\<^sub>i\<^sub>r]"
-    by (metis apply_r_upd.simps)
-  then have "val_epoch_state (apply_r_upd (create_r_upd b s\<^sub>1) s\<^sub>2) =
+      and f2: "unregistered = fmdom' stk_creds \<lhd>/ i\<^sub>r\<^sub>w\<^sub>d"
+      and f3: "non_distributed = (\<Sum>k \<in> fmdom' unregistered. unregistered $$! k)"
+      and f4: "rew'\<^sub>m\<^sub>i\<^sub>r = fmdom' stk_creds \<lhd> i\<^sub>r\<^sub>w\<^sub>d"
+      and f5: "update\<^sub>r\<^sub>w\<^sub>d = fmap_of_list [(addr_rwd hk, val). (hk, val) \<leftarrow> sorted_list_of_fmap rew'\<^sub>m\<^sub>i\<^sub>r]"
+      by (metis apply_r_upd.simps)
+  then have "val_epoch_state (apply_r_upd ru es) =
     treasury + reserves + val_utxo utxo + deps + fees + val_map rewards + \<Delta>t + \<Delta>r + non_distributed
     + \<Delta>f + val_map rs + val_map update\<^sub>r\<^sub>w\<^sub>d"
   proof -
-    from f1 and f3 have "val_epoch_state (apply_r_upd (create_r_upd b s\<^sub>1) s\<^sub>2) =
+    from assms(1) and f1 have "val_epoch_state (apply_r_upd ru es) =
       val_acnt (treasury + \<Delta>t, reserves + \<Delta>r + non_distributed)
       + val_ledger_state (
         (utxo, deps, fees + \<Delta>f, up), ((stk_creds, (rewards \<union>\<^sub>+ rs) \<union>\<^sub>+ update\<^sub>r\<^sub>w\<^sub>d, {$$}), pstate))"
       by simp
-    then have "val_epoch_state (apply_r_upd (create_r_upd b s\<^sub>1) s\<^sub>2) =
+    then have "val_epoch_state (apply_r_upd ru es) =
       (treasury + \<Delta>t) + (reserves + \<Delta>r + non_distributed) + val_utxo utxo + deps + (fees + \<Delta>f)
       + val_map ((rewards \<union>\<^sub>+ rs) \<union>\<^sub>+ update\<^sub>r\<^sub>w\<^sub>d)"
       by auto
@@ -807,42 +805,11 @@ proof -
       by linarith
   qed
   moreover have "\<Delta>t + \<Delta>r + non_distributed + \<Delta>f + val_map rs + val_map update\<^sub>r\<^sub>w\<^sub>d = 0"
-  proof (cases ss\<^sub>1)
-    case (fields pstake\<^sub>m\<^sub>a\<^sub>r\<^sub>k pstake\<^sub>s\<^sub>e\<^sub>t pstake\<^sub>g\<^sub>o pools_ss fee_ss)
-    from f0 and fields have "s\<^sub>1 =
-      (
-        (treasury\<^sub>1, reserves\<^sub>1),
-        (pstake\<^sub>m\<^sub>a\<^sub>r\<^sub>k, pstake\<^sub>s\<^sub>e\<^sub>t, pstake\<^sub>g\<^sub>o, pools_ss, fee_ss),
-        ((utxo\<^sub>1, deps\<^sub>1, fees\<^sub>1, up\<^sub>1), (stk_creds\<^sub>1, rewards\<^sub>1, i\<^sub>r\<^sub>w\<^sub>d), pstate\<^sub>1),
-        ppm\<^sub>1
-      )"
+  proof -
+    from assms(4-6) have "\<Delta>t + \<Delta>r + non_distributed + \<Delta>f + val_map rs + val_map update\<^sub>r\<^sub>w\<^sub>d =
+      \<Delta>t - \<Delta>r\<^sub>l - val_map i\<^sub>r\<^sub>w\<^sub>d + non_distributed + \<Delta>f + val_map rs + val_map update\<^sub>r\<^sub>w\<^sub>d"
       by simp
-    then obtain \<Delta>t\<^sub>1 \<Delta>t\<^sub>2 \<Delta>r' \<Delta>r\<^sub>l rs' rewards\<^sub>m\<^sub>i\<^sub>r reward_pot R
-      where "create_r_upd b s\<^sub>1 = (\<Delta>t\<^sub>1 + \<Delta>t\<^sub>2, -\<Delta>r', rs', -fee_ss, i\<^sub>r\<^sub>w\<^sub>d)"
-      and "rewards\<^sub>m\<^sub>i\<^sub>r = (\<Sum> k \<in> fmdom' i\<^sub>r\<^sub>w\<^sub>d. i\<^sub>r\<^sub>w\<^sub>d $$! k)"
-      and "reward_pot = fee_ss + \<Delta>r\<^sub>l"
-      and "R = reward_pot - \<Delta>t\<^sub>1"
-      and "\<Delta>t\<^sub>2 = R - (\<Sum> k \<in> fmdom' rs'. rs' $$! k)"
-      and "\<Delta>r' = \<Delta>r\<^sub>l + rewards\<^sub>m\<^sub>i\<^sub>r"
-      by (metis create_r_upd.simps prod.exhaust_sel that)
-    with f1 and f2 and fields have "rs' = rs" and "\<Delta>r' = -\<Delta>r" and "\<Delta>t = \<Delta>t\<^sub>1 + \<Delta>t\<^sub>2"
-      and "\<Delta>f = -fee_ss"
-      by auto
-    with \<open>R = reward_pot - \<Delta>t\<^sub>1\<close> and \<open>\<Delta>t\<^sub>2 = R - val_map rs'\<close> and \<open>reward_pot = fee_ss + \<Delta>r\<^sub>l\<close>
-    have "\<Delta>t\<^sub>1 + \<Delta>t\<^sub>2 - \<Delta>r\<^sub>l + val_map rs - fee_ss = 0"
-      by simp
-    from \<open>\<Delta>t = \<Delta>t\<^sub>1 + \<Delta>t\<^sub>2\<close> have "\<Delta>t + \<Delta>r + non_distributed + \<Delta>f + val_map rs + val_map update\<^sub>r\<^sub>w\<^sub>d =
-      \<Delta>t\<^sub>1 + \<Delta>t\<^sub>2 + \<Delta>r + non_distributed + \<Delta>f + val_map rs + val_map update\<^sub>r\<^sub>w\<^sub>d"
-      by simp
-    also from \<open>\<Delta>r' = \<Delta>r\<^sub>l + rewards\<^sub>m\<^sub>i\<^sub>r\<close> and \<open>\<Delta>r' = -\<Delta>r\<close> and \<open>rewards\<^sub>m\<^sub>i\<^sub>r = val_map i\<^sub>r\<^sub>w\<^sub>d\<close>
-    have "\<dots> = \<Delta>t\<^sub>1 + \<Delta>t\<^sub>2 - \<Delta>r\<^sub>l - val_map i\<^sub>r\<^sub>w\<^sub>d + non_distributed + \<Delta>f + val_map rs
-      + val_map update\<^sub>r\<^sub>w\<^sub>d"
-      by simp
-    also from \<open>\<Delta>f = -fee_ss\<close> have "\<dots> = \<Delta>t\<^sub>1 + \<Delta>t\<^sub>2 - \<Delta>r\<^sub>l + val_map rs - fee_ss - val_map i\<^sub>r\<^sub>w\<^sub>d
-      + non_distributed + val_map update\<^sub>r\<^sub>w\<^sub>d"
-      by simp
-    also from \<open>\<Delta>t\<^sub>1 + \<Delta>t\<^sub>2 - \<Delta>r\<^sub>l + val_map rs - fee_ss = 0\<close> have "\<dots> =
-      - val_map i\<^sub>r\<^sub>w\<^sub>d + non_distributed + val_map update\<^sub>r\<^sub>w\<^sub>d"
+    also from assms(3,6) have "\<dots> = - val_map i\<^sub>r\<^sub>w\<^sub>d + non_distributed + val_map update\<^sub>r\<^sub>w\<^sub>d"
       by simp
     also have "\<dots> = 0"
     proof -
@@ -850,26 +817,27 @@ proof -
       proof -
         have "val_map rew'\<^sub>m\<^sub>i\<^sub>r + val_map unregistered = val_map update\<^sub>r\<^sub>w\<^sub>d + non_distributed"
         proof -
-          from f6 and assms(1,2) have "val_map rew'\<^sub>m\<^sub>i\<^sub>r = val_map update\<^sub>r\<^sub>w\<^sub>d"
+          from f5 and assms(7,8) have "val_map rew'\<^sub>m\<^sub>i\<^sub>r = val_map update\<^sub>r\<^sub>w\<^sub>d"
             by (simp add: val_map_fmap_of_list)
-          moreover from f4 and f7 have "val_map unregistered = non_distributed"
+          moreover from f2 and f3 have "val_map unregistered = non_distributed"
             by simp
           ultimately show ?thesis
             by simp
         qed
-        moreover from f5 and f7 have "val_map i\<^sub>r\<^sub>w\<^sub>d = val_map rew'\<^sub>m\<^sub>i\<^sub>r + val_map unregistered"
+        moreover from assms(3) and f2 and f4 have "val_map i\<^sub>r\<^sub>w\<^sub>d =
+          val_map rew'\<^sub>m\<^sub>i\<^sub>r + val_map unregistered"
           using val_map_split by (metis add.commute)
         ultimately show ?thesis
           by simp
       qed
       then show ?thesis
         by simp
-  qed
+    qed
     finally show ?thesis .
   qed
-  moreover have "val_epoch_state s\<^sub>2 =
+  moreover from f0 have "val_epoch_state es =
     treasury + reserves + val_utxo utxo + deps + fees + val_map rewards"
-    using f2 by simp
+    by simp
   ultimately show ?thesis
     by simp
 qed
@@ -1103,12 +1071,20 @@ lemma newepoch_value_preservation:
 proof -
   from assms show ?thesis
   proof cases
-    case (new_epoch e\<^sub>l ru ru' _ _ _ _ i\<^sub>r\<^sub>w\<^sub>d' es b\<^sub>p\<^sub>r\<^sub>e\<^sub>v es' es'' pd' osched' b\<^sub>c\<^sub>u\<^sub>r pd osched)
+    case (new_epoch e\<^sub>l ru ru' \<Delta>t \<Delta>r rs \<Delta>f i\<^sub>r\<^sub>w\<^sub>d es rewards\<^sub>m\<^sub>i\<^sub>r \<Delta>r\<^sub>l es' es'' pd' osched' b\<^sub>p\<^sub>r\<^sub>e\<^sub>v b\<^sub>c\<^sub>u\<^sub>r pd osched)
     have "val_epoch_state es'' = val_epoch_state es"
     proof -
-      from \<open>inj addr_rwd\<close> and \<open>mono addr_rwd\<close> and \<open>ru' = create_r_upd b\<^sub>p\<^sub>r\<^sub>e\<^sub>v es\<close> have "
+      from
+        \<open>inj addr_rwd\<close> and
+        \<open>mono addr_rwd\<close> and
+        \<open>(\<Delta>t, \<Delta>r, rs, \<Delta>f, i\<^sub>r\<^sub>w\<^sub>d) = ru'\<close> and
+        \<open>i\<^sub>r\<^sub>w\<^sub>d = get_ir es\<close> and
+        \<open>\<Delta>f = - get_fee_ss es\<close> and
+        \<open>rewards\<^sub>m\<^sub>i\<^sub>r = (\<Sum> k \<in> fmdom' i\<^sub>r\<^sub>w\<^sub>d. i\<^sub>r\<^sub>w\<^sub>d $$! k)\<close> and
+        \<open>- \<Delta>r = \<Delta>r\<^sub>l + rewards\<^sub>m\<^sub>i\<^sub>r\<close> and
+        \<open>\<Delta>t - \<Delta>r\<^sub>l + (\<Sum> k \<in> fmdom' rs. rs $$! k) + \<Delta>f = 0\<close> have "
         val_epoch_state (apply_r_upd ru' es) = val_epoch_state es"
-        using reward_update_value_preservation by presburger
+        using reward_update_application_value_preservation by simp
       with \<open>es' = apply_r_upd ru' es\<close> and \<open>\<turnstile> es' \<rightarrow>\<^bsub>EPOCH\<^esub>{\<epsilon>} es''\<close> show ?thesis
         using epoch_value_preservation by simp
     qed
@@ -1117,10 +1093,12 @@ proof -
       by simp
   next
     case not_new_epoch
-    then show ?thesis by simp
+    then show ?thesis
+      by simp
   next
     case no_reward_update
-    then show ?thesis by simp
+    then show ?thesis
+      by simp
   qed
 qed
 
